vec2 spec

specs/Spec.Chacha20_vec2.fst
@@ -1,4 +1,4 @@
-module Spec.Chacha20
+module Spec.Chacha20_vec2
 
 open FStar.Mul
 open FStar.Seq
@@ -6,9 +6,10 @@ open FStar.UInt32
 open FStar.Endianness
 open Spec.Lib
 
+module U32 = FStar.UInt32
 (* This should go elsewhere! *)
 
-#set-options "--initial_fuel 0 --max_fuel 0 --z3rlimit 100"
+#set-options "--initial_fuel 0 --max_fuel 0 --initial_ifuel 0 --max_ifuel 0 --z3rlimit 100"
 
 let keylen = 32 (* in bytes *)
 let blocklen = 64  (* in bytes *)
@@ -19,11 +20,35 @@ type block = lbytes blocklen
 type nonce = lbytes noncelen
 type counter = UInt.uint_t 32
 
-// using @ as a functional substitute for ;
-// internally, blocks are represented as 16 x 4-byte integers
-type state = m:seq UInt32.t {length m = 16}
-type idx = n:nat{n < 16}
+// What we need to know about vectors:
+type vec   = v:seq UInt32.t {length v = 8}
+let to_vec (x:U32.t) : vec = create 8 x
+type state = m:seq vec      {length m = 16}
+type idx = n:nat{n < 4}
 type shuffle = state -> Tot state 
+
+
+// Vector size changes the blocksize and the counter step:
+type vec_block = lbytes (8*blocklen)
+unfold let counter_step:vec  = to_vec 8ul
+unfold let initial_counter : vec = 
+       let l = [0ul; 1ul; 2ul; 3ul; 4ul; 5ul; 6ul; 7ul] in
+       assert_norm(List.Tot.length l = 8); 
+       let s = createL l in
+       s       
+//Transposed state matrix
+type stateT = m:seq (r:seq U32.t{length r = 16}){length m = 8}
+
+//Chacha20 code begins
+
+unfold let op_Plus_Percent_Hat (x:vec) (y:vec) : Tot vec = 
+       Combinators.seq_map2 U32.op_Plus_Percent_Hat x y
+
+unfold let op_Hat_Hat (x:vec) (y:vec) : Tot vec = 
+       Combinators.seq_map2 U32.op_Hat_Hat x y
+
+unfold let op_Less_Less_Less (x:vec) (n:UInt32.t{v n < 32}) : Tot vec = 
+       Combinators.seq_map (fun x -> x <<< n) x 
 
 val line: idx -> idx -> idx -> s:UInt32.t {v s < 32} -> shuffle
 let line a b d s m = 
@@ -31,61 +56,101 @@ let line a b d s m =
   let m = upd m d ((index m d ^^  index m a) <<< s) in
   m
 
-let quarter_round a b c d : shuffle = 
-  line a b d 16ul @ 
-  line c d b 12ul @
-  line a b d 8ul @ 
-  line c d b 7ul 
+let column_round : shuffle =
+  line 0 8 12 16ul @
+  line 1 9 13 16ul @
+  line 2 10 14 16ul @
+  line 3 11 15 16ul @
 
-let column_round : shuffle = 
-  quarter_round 0 4 8 12 @
-  quarter_round 1 5 9 13 @
-  quarter_round 2 6 10 14 @
-  quarter_round 3 7 11 15
+  line 8 12 4 12ul @
+  line 9 13 5 12ul @
+  line 10 14 6 12ul @
+  line 11 15 7 12ul @
 
-let diagonal_round : shuffle = 
-  quarter_round 0 5 10 15 @
-  quarter_round 1 6 11 12 @
-  quarter_round 2 7 8 13 @
-  quarter_round 3 4 9 14
+  line 0 8 12 8ul @
+  line 1 9 13 8ul @
+  line 2 10 14 8ul @
+  line 3 11 15 8ul @
 
-let double_round: shuffle = 
-    column_round @ diagonal_round (* 2 rounds *)
+  line 8 12 4 7ul @
+  line 9 13 5 7ul @
+  line 10 14 6 7ul @
+  line 11 15 7 7ul 
+
+let diagonal_round : shuffle =
+  line 0 5 15 16ul @
+  line 1 6 12 16ul @
+  line 2 7 13 16ul @
+  line 3 4 14 16ul @
+
+  line 10 15 5 12ul @
+  line 11 12 6 12ul @
+  line 8 13 7 12ul @
+  line 9 14 4 12ul @
+
+  line 0 5 15 8ul @
+  line 1 6 12 8ul @
+  line 2 7 13 8ul @
+  line 3 4 14 8ul @
+
+  line 10 15 5 7ul @
+  line 11 12 6 7ul @
+  line 8 13 7 7ul @
+  line 9 14 4 7ul 
+
+let double_round : shuffle =
+  column_round @ diagonal_round
 
 let rounds : shuffle = 
     iter 10 double_round (* 20 rounds *)
 
 let chacha20_core (s:state) : Tot state = 
     let s' = rounds s in
-    map2 (fun x y -> x +%^ y) s' s
+    Combinators.seq_map2 op_Plus_Percent_Hat s' s
 
 (* state initialization *) 
 
-unfold let constants = [0x61707865ul; 0x3320646eul; 0x79622d32ul; 0x6b206574ul]
+unfold let constants : (s:seq U32.t{length s = 4}) = 
+       let l = [0x61707865ul; 0x3320646eul; 0x79622d32ul; 0x6b206574ul] in
+         assert_norm(List.Tot.length l = 4);
+	 createL l	 
 
-// JK: I have to add those assertions to typechecks, would be nice to get rid of it
 let setup (k:key) (n:nonce) (c:counter): Tot state =
-  assert_norm(List.Tot.length constants = 4); assert_norm(List.Tot.length [UInt32.uint_to_t c] = 1);
-  createL constants @|
-  uint32s_from_le 8 k @|
-  singleton (UInt32.uint_to_t c) @|
-  (* create [UInt32.uint_to_t c] @|  *)
-  uint32s_from_le 3 n
+  let constants:seq vec = Combinators.seq_map to_vec constants in
+  let key = Combinators.seq_map to_vec (uint32s_from_le 8 k) in
+  let nonce = Combinators.seq_map to_vec (uint32s_from_le 3 n) in
+  let ctr = create 1 initial_counter in
+  constants @| key @| ctr @| nonce
 
-let chacha20_block (k:key) (n:nonce) (c:counter): Tot block =
+let transpose (s:state): Tot stateT =
+    let cols = createL [0;1;2;3;4;5;6;7] in
+    Combinators.seq_map (fun i -> Combinators.seq_map (fun r -> index r i) s) cols
+
+let state_to_key (s:state): Tot vec_block =
+    let k = transpose s in
+    uint32s_to_le 16 (index k 0) @|
+    uint32s_to_le 16 (index k 1) @|
+    uint32s_to_le 16 (index k 2) @|
+    uint32s_to_le 16 (index k 3) @|
+    uint32s_to_le 16 (index k 4) @|
+    uint32s_to_le 16 (index k 5) @|
+    uint32s_to_le 16 (index k 6) @|
+    uint32s_to_le 16 (index k 7) 
+
+
+let chacha20_block (k:key) (n:nonce) (c:counter): Tot vec_block =
     let st = setup k n c in
     let st' = chacha20_core st in
-    uint32s_to_le 16 st'
-
+    state_to_key st'    
 
 let chacha20_ctx: Spec.CTR.block_cipher_ctx = 
     let open Spec.CTR in
     {
     keylen = keylen;
-    blocklen = blocklen;
+    blocklen = 8 * blocklen;
     noncelen = noncelen;
     counterbits = 32;
-    incr = 1
+    incr = 8
     }
 
 let chacha20_cipher: Spec.CTR.block_cipher chacha20_ctx = chacha20_block
